aneris/examples/snapshot_isolation/examples/classical_example/classical_example_proof.v
@@ -195,9 +195,9 @@ Context `{!anerisG Mdl Σ, !SI_resources Mdl Σ, !SI_client_toolbox}.
     { iNext. iExists h. iFrame. }
     iModIntro. wp_pures.
     wp_apply (SI_read_spec $! _ _ _ _ with "[] [Hcx]"); try set_solver.
-    iFrame. iIntros (vx) "(Hcx & %hx_vx)". wp_pures.
+    iFrame. iIntros "Hcx". wp_pures.
     wp_apply (SI_read_spec $! _ _ _ _ with "[] [Hcy]"); try set_solver.
-    iFrame. iIntros (vy) "(Hcy & %hy_vy)". wp_pures.
+    iFrame. iIntros "Hcy". wp_pures.
     destruct (hist_val h); wp_pures; do 2 wp_lam; wp_pures.
       - case_bool_decide as Heq; try set_solver. wp_pures. 
       wp_apply (commitU_spec rpc client_3_addr (⊤ ∖ ↑client_inv_name));
@@ -278,7 +278,7 @@ Context `{!anerisG Mdl Σ, !SI_init}.
       example_runner @["system"]
     {{{ v, RET v; True }}}.
   Proof.
-    iMod (SI_init_module $! (I: True)) as (SI_res SI_client_toolbox) "(HKVSres & HVKSinit)".
+    iMod SI_init_module as (SI_res SI_client_toolbox) "(HKVSres & HVKSinit)".
     iMod (inv_alloc client_inv_name ⊤ (client_inv) with "[HKVSres]") as "#Hinv".
     { iNext. iExists [].
     iDestruct (big_sepS_delete _ _ "x" with "HKVSres") as "(Hx & HKVSres)";
